Removed Typeclasses, shifted everything to functions

helper.fst
@@ -1,22 +1,6 @@
 module Helper
 
 open FStar.List.Tot
-open FStar.Tactics.Typeclasses
-open FStar.Tactics
-
-(*
-Things to be moved here:
-+ func member
-+ func unique
-+ type ae
-- Props for diff
-- Props for union
-- Props for abs_merge, merge and prop_merge
-
-All of these, depend on types op and o which are specific to each MRDT.
-One thing we can do is create an init function, that takes in the op and returns the MRDT-specific funcs and props.
-I'm thinking of other ideas still. If I come up with anything cleaner, I'll add that.
-*)
 
 val member : #op:eqtype
            -> id:nat
@@ -28,7 +12,6 @@ let rec member n l =
   |[] -> false
   |(id,_)::xs -> (n = id) || member n xs
 
-// type v = (o:eqtype{exists op. subtype_of o (nat * op)})
 
 val unique : #op:eqtype
            -> l:list (nat * op)
@@ -43,23 +26,20 @@ let get_id (id,_) = id
 let get_op (_,op) = op
 
 noeq type ae (op:eqtype) =
-| A : vis : ((nat * op) -> (nat * op) -> Tot bool)
-      ->  l:(list (nat * op)) {(forall e e' e''. (mem e l /\ mem e' l /\ mem e'' l  /\ get_id e <> get_id e' /\ 
-                         get_id e' <> get_id e'' /\ get_id e <> get_id e'  /\ vis e e' /\ vis e' e'') ==> vis e e'') /\
-                      (forall e e'. (mem e l /\ mem e' l /\ get_id e <> get_id e' /\  vis e e') ==> not (vis e' e)) /\
-                      (forall e. mem e l ==> not (vis e e) /\
-                      (unique l))}
-      ->  ae op
+|A : vis : ((nat * op) -> (nat * op) -> Tot bool) -> l:list (nat * op) {unique l} -> ae op
 
-class mrdt_props (op:eqtype) (s:eqtype) (app_op:s -> (nat * op) -> s) (sim_prop:s -> (ae op) ->s -> bool -> prop) (diff_prop:prop) (union_prop:prop)  = {
+assume val axiom : op: eqtype -> l:ae op
+                 -> Lemma (ensures (forall e e' e''. (mem e l.l /\ mem e' l.l /\ mem e'' l.l /\ get_id e <> get_id e' /\
+                         get_id e' <> get_id e'' /\ get_id e <> get_id e'' /\ l.vis e e' /\ l.vis e' e'') ==> l.vis e e'') (*transitive*)/\
+                         (forall e e'. (mem e l.l /\ mem e' l.l /\ get_id e <> get_id e' /\ l.vis e e') ==> not (l.vis e' e)) (*asymmetric*) /\
+                         (forall e. mem e l.l ==> not (l.vis e e) (*irreflexive*)))
+                         [SMTPat (unique l.l)]
 
-  sim : s0:s
-        -> tr:ae op
-        -> s1:s
-        -> Tot (b:bool{ sim_prop s0 tr s1 b });
-
-
-  absmerge : l:ae op
+let sim_type (op:eqtype) (s:eqtype) (sim_prop:s -> (ae op) ->s -> bool -> prop) =  s0:s
+                                                                               -> tr:ae op
+                                                                               -> s1:s
+                                                                               -> Tot (b:bool{ sim_prop s0 tr s1 b })
+let abs_merge_type (op:eqtype) = l:ae op
              -> a:ae op
              -> b:ae op
              -> Pure (ae op)
@@ -72,9 +52,9 @@ class mrdt_props (op:eqtype) (s:eqtype) (app_op:s -> (nat * op) -> s) (sim_prop:
                                           (mem e1 a.l /\ mem e2 a.l /\ get_id e1 <> get_id e2 /\ a.vis e1 e2) \/
                                           (mem e1 b.l /\ mem e2 b.l /\ get_id e1 <> get_id e2 /\ b.vis e1 e2) \/
                                           (mem e1 l.l /\ mem e2 a.l /\ get_id e1 <> get_id e2) \/
-                                          (mem e1 l.l /\ mem e2 b.l /\ get_id e1 <> get_id e2))));
+                                          (mem e1 l.l /\ mem e2 b.l /\ get_id e1 <> get_id e2))))
 
-  merge : s0:s
+let merge_type (op:eqtype) (s:eqtype) (sim_prop: s -> (ae op) -> s -> bool -> prop) (sim: (s0:s) -> (tr:ae op)  -> (s1:s) -> Tot (b:bool{ sim_prop s0 tr s1 b })) = s0:s
           -> ltr:ae op
           -> l:s
           -> atr:ae op
@@ -85,9 +65,29 @@ class mrdt_props (op:eqtype) (s:eqtype) (app_op:s -> (nat * op) -> s) (sim_prop:
                              (forall e. mem e ltr.l ==> not (member (get_id e) atr.l)) /\
                              (forall e. mem e atr.l ==> not (member (get_id e) btr.l)) /\
                              (forall e. mem e btr.l ==> not (member (get_id e) ltr.l)))
-                   (ensures (fun res -> true));
+                   (ensures (fun res -> true))
 
-  prop_merge : s0:s
+let prop_merge_type (op:eqtype) (s:eqtype) (sim_prop: s -> (ae op) -> s -> bool -> prop) 
+                    (sim: (s0:s) -> (tr:ae op)  -> (s1:s) -> Tot (b:bool{ sim_prop s0 tr s1 b })) 
+                      (merge : (s0:s) -> (ltr: ae op) -> (l:s) -> (atr:ae op) -> (a:s) -> (btr:ae op) -> (b:s)
+                             -> Pure s (requires (sim s0 ltr l /\ sim l atr a /\ sim l btr b) /\
+                             (forall e. mem e ltr.l ==> not (member (get_id e) atr.l)) /\
+                             (forall e. mem e atr.l ==> not (member (get_id e) btr.l)) /\
+                             (forall e. mem e btr.l ==> not (member (get_id e) ltr.l)))
+                             (ensures (fun res -> true)))
+                       (absmerge : (l:ae op) -> (a:ae op) -> (b:ae op) 
+                                 -> Pure (ae op)
+                                 (requires (forall e. mem e l.l ==> not (member (get_id e) a.l)) /\
+                                 (forall e. mem e a.l ==> not (member (get_id e) b.l)) /\
+                                 (forall e. mem e b.l ==> not (member (get_id e) l.l)))
+                                 (ensures (fun u -> (forall e. mem e u.l <==> mem e l.l \/ mem e a.l \/ mem e b.l) /\
+                                   (forall e1 e2. (mem e1 u.l /\ mem e2 u.l /\ get_id e1 <> get_id e2 /\ u.vis e1 e2) <==>
+                                          (mem e1 l.l /\ mem e2 l.l /\ get_id e1 <> get_id e2 /\ l.vis e1 e2) \/
+                                          (mem e1 a.l /\ mem e2 a.l /\ get_id e1 <> get_id e2 /\ a.vis e1 e2) \/
+                                          (mem e1 b.l /\ mem e2 b.l /\ get_id e1 <> get_id e2 /\ b.vis e1 e2) \/
+                                          (mem e1 l.l /\ mem e2 a.l /\ get_id e1 <> get_id e2) \/
+                                          (mem e1 l.l /\ mem e2 b.l /\ get_id e1 <> get_id e2)))))
+               = s0:s
                -> ltr:ae op
                -> l:s
                -> atr:ae op
@@ -98,62 +98,32 @@ class mrdt_props (op:eqtype) (s:eqtype) (app_op:s -> (nat * op) -> s) (sim_prop:
                                  (forall e. mem e ltr.l ==> not (member (get_id e) atr.l)) /\
                                  (forall e. mem e atr.l ==> not (member (get_id e) btr.l)) /\
                                  (forall e. mem e btr.l ==> not (member (get_id e) ltr.l)))
-                       (ensures (sim s0 (absmerge ltr atr btr) (merge s0 ltr l atr a btr b)));
+                       (ensures (sim s0 (absmerge ltr atr btr) (merge s0 ltr l atr a btr b)))
 
- append : tr:ae op
+let append_type (op:eqtype) = tr:ae op
            -> o:(nat * op)
            -> Pure (ae op)
              (requires (not (member (get_id o) tr.l)))
              (ensures (fun res -> (forall e. mem e res.l <==> mem e tr.l \/ e = o) /\
                                (forall e1 e2. (mem e1 res.l /\ mem e2 res.l /\ get_id e1 <> get_id e2 /\ res.vis e1 e2) <==>
                                          (mem e1 tr.l /\ mem e2 tr.l /\ get_id e1 <> get_id e2 /\ tr.vis e1 e2) \/
-                                         (mem e1 tr.l /\ e2 = o /\ get_id e1 <> get_id e2))));
+                                         (mem e1 tr.l /\ e2 = o /\ get_id e1 <> get_id e2))))
 
- prop_oper : s0:s
+let prop_oper_type (op:eqtype) (s:eqtype) (app_op:s -> (nat * op) -> s) (sim_prop: s -> (ae op) -> s -> bool -> prop)
+                    (sim: (s0:s) -> (tr:ae op)  -> (s1:s) -> Tot (b:bool{ sim_prop s0 tr s1 b }))
+                    (append: (tr:ae op) -> (o:(nat * op))
+                             -> Pure (ae op)
+                             (requires (not (member (get_id o) tr.l)))
+                             (ensures (fun res -> (forall e. mem e res.l <==> mem e tr.l \/ e = o) /\
+                               (forall e1 e2. (mem e1 res.l /\ mem e2 res.l /\ get_id e1 <> get_id e2 /\ res.vis e1 e2) <==>
+                                         (mem e1 tr.l /\ mem e2 tr.l /\ get_id e1 <> get_id e2 /\ tr.vis e1 e2) \/
+                                         (mem e1 tr.l /\ e2 = o /\ get_id e1 <> get_id e2)))))
+              = s0:s
               -> tr:ae op
               -> st:s
               -> op:(nat * op)
               -> Lemma (requires (sim s0 tr st) /\
                                 (not (member (get_id op) tr.l)) /\
                                 (forall e. mem e tr.l ==> mem op (append tr op).l /\ (append tr op).vis e op))
-                      (ensures (sim s0 (append tr op) (app_op st op)));
+                      (ensures (sim s0 (append tr op) (app_op st op)))
 
- convergence : s0:s
-                -> tr:ae op
-                -> a:s
-                -> b:s
-                -> Lemma (requires (sim s0 tr a /\ sim s0 tr b))
-                        (ensures (a = b));
-
- // diff : a:ae op
- //         -> l:ae op
- //         -> Pure (ae op)
- //          (requires (forall e. mem e l.l ==> mem e a.l) /\
- //                    (forall e e1. mem e l.l /\ mem e1 l.l /\ l.vis e e1 ==> mem e a.l /\ mem e1 a.l /\ a.vis e e1) /\
- //                    (forall e e1. (mem e l.l /\ mem e1 a.l ==> mem e a.l /\ a.vis e e1)))
- //          (ensures (fun d -> (forall e. mem e d.l <==> mem e a.l /\ not(mem e l.l)) /\
- //                          (forall e. mem e d.l ==> not (member (get_id e) l.l)) /\
- //                          (diff_prop) /\
- //                          (forall e e1. mem e d.l /\ mem e1 d.l /\ d.vis e e1 ==> mem e a.l /\ mem e1 a.l /\ a.vis e e1) /\
- //                          (forall e e1. (mem e d.l /\ mem e1 d.l /\ not (d.vis e e1)) ==> (mem e a.l /\ mem e1 a.l /\ not (a.vis e e1))) /\
- //                          (forall e e1. (mem e d.l /\ mem e1 d.l /\ not (d.vis e e1 || d.vis e1 e)) ==>
- //                                   (mem e a.l /\ mem e1 a.l /\ not (a.vis e e1 || a.vis e1 e))))) (decreases l);
-
- //  union :  a:ae op
- //          -> b:ae op
- //          -> Pure (ae op)
- //            (requires (forall e. (mem e a.l ==> not (member (get_id e) b.l))) /\
- //                            (forall e. (mem e b.l ==> not (member (get_id e) a.l))))
- //            (ensures (fun u ->
- //                            (forall e. mem e u.l <==> mem e a.l \/ mem e b.l) /\
- //                            (union_prop) /\
- //                            (forall e e1. (mem e u.l /\ mem e1 u.l /\ u.vis e e1) <==>
- //                                     ((mem e a.l /\ mem e1 a.l /\ a.vis e e1) \/ (mem e b.l /\ mem e1 b.l /\ b.vis e e1))) /\
- //                            (forall e e1. mem e a.l /\ mem e1 a.l /\ not (a.vis e e1) ==> mem e u.l /\ mem e1 u.l /\ not (u.vis e e1)) /\
- //                            (forall e e1. mem e b.l /\ mem e1 b.l /\ not (b.vis e e1) ==> mem e u.l /\ mem e1 u.l /\ not (u.vis e e1)) /\
- //                            (forall e e1. mem e a.l /\ mem e1 a.l /\ not (a.vis e e1 || a.vis e1 e) ==>
- //                                     mem e u.l /\ mem e1 u.l /\ not (u.vis e e1 || u.vis e1 e)) /\
- //                            (forall e e1. mem e b.l /\ mem e1 b.l /\ not (b.vis e e1 || b.vis e1 e) ==>
- //                                     mem e u.l /\ mem e1 u.l /\ not (u.vis e e1 || u.vis e1 e))))
-
-}
